move pts_to_witinv to .fst

ulib/experimental/Steel.C.Ref.fsti
@@ -32,7 +32,7 @@ val ref_focus
 : ref a q
 
 val ref_focus_id
-  (#a:Type) (#b:Type) (#c:Type) (#p: pcm b)
+  (#a:Type) (#b:Type) (#p: pcm b)
   (r: ref a p)
 : Lemma
   (ref_focus r (connection_id _) == r)
@@ -190,81 +190,21 @@ let sel_view_inv
   in
   ()
 
-let pts_to_view_explicit
+val pts_to_view_sl
   (#a: Type u#0) (#b: Type u#b) (#p: pcm b)
   (r: ref a p)
   (#c: Type u#c)
   (#can_view_unit: bool)
   (vw: sel_view p c can_view_unit)
-  (v: Ghost.erased c)
-: Tot M.slprop
-= hp_of (pts_to r (vw.to_carrier v))
+: Tot (M.slprop u#1)
 
-val pts_to_view_explicit_witinv
-  (#a: Type u#0) (#b: Type u#b) (#p: pcm b)
-  (r: ref a p)
-  (#c: Type u#c)
-  (#can_view_unit: bool)
-  (vw: sel_view p c can_view_unit)
-: Lemma
-  (M.is_witness_invariant (pts_to_view_explicit r vw))
-
-let pts_to_view_sl
-  (#a: Type u#0) (#b: Type u#b) (#p: pcm b)
-  (r: ref a p)
-  (#c: Type u#c)
-  (#can_view_unit: bool)
-  (vw: sel_view p c can_view_unit)
-: Tot M.slprop
-= M.h_exists (pts_to_view_explicit r vw)
-
-let pts_to_view_sel'
-  (#a: Type u#0) (#b: Type u#b) (#p: pcm b)
-  (r: ref a p)
-  (#c: Type0)
-  (#can_view_unit: bool)
-  (vw: sel_view p c can_view_unit)
-: Tot (selector' c (pts_to_view_sl r vw))
-= fun h ->
-  let x = M.id_elim_exists #(Ghost.erased c) (pts_to_view_explicit r vw) h in
-  Ghost.reveal (Ghost.reveal x)
-
-let pts_to_view_depends_only_on
-  (#a: Type u#0) (#b: Type u#b) (#p: pcm b)
-  (r: ref a p)
-  (#c: Type0)
-  (#can_view_unit: bool)
-  (vw: sel_view p c can_view_unit)
-  (m0:M.hmem (pts_to_view_sl r vw)) (m1:M.mem{M.disjoint m0 m1})
-: Lemma (pts_to_view_sel' r vw m0 == pts_to_view_sel' r vw (M.join m0 m1))
-= let x = Ghost.reveal (M.id_elim_exists #(Ghost.erased c) (pts_to_view_explicit r vw) m0) in
-  let y = Ghost.reveal (M.id_elim_exists #(Ghost.erased c) (pts_to_view_explicit r vw) (M.join m0 m1)) in
-  pts_to_view_explicit_witinv r vw;
-  M.elim_wi (pts_to_view_explicit r vw) x y (M.join m0 m1)
-
-let pts_to_view_depends_only_on_core
-  (#a: Type u#0) (#b: Type u#b) (#p: pcm b)
-  (r: ref a p)
-  (#c: Type0)
-  (#can_view_unit: bool)
-  (vw: sel_view p c can_view_unit)
-  (m0:M.hmem (pts_to_view_sl r vw))
-: Lemma (pts_to_view_sel' r vw m0 == pts_to_view_sel' r vw (M.core_mem m0))
-= let x = Ghost.reveal (M.id_elim_exists #(Ghost.erased c) (pts_to_view_explicit r vw) m0) in
-  let y = Ghost.reveal (M.id_elim_exists #(Ghost.erased c) (pts_to_view_explicit r vw) (M.core_mem m0)) in
-  pts_to_view_explicit_witinv r vw;
-  M.elim_wi (pts_to_view_explicit r vw) x y (M.core_mem m0)
-
-let pts_to_view_sel
+val pts_to_view_sel
   (#a: Type u#0) (#b: Type u#b) (#p: pcm b)
   (r: ref a p)
   (#c: Type0)
   (#can_view_unit: bool)
   (vw: sel_view p c can_view_unit)
 : Tot (selector c (pts_to_view_sl r vw))
-= Classical.forall_intro_2 (pts_to_view_depends_only_on r vw);
-  Classical.forall_intro (pts_to_view_depends_only_on_core r vw);
-  pts_to_view_sel' r vw
 
 [@@__steel_reduce__]
 let pts_to_view'
@@ -295,26 +235,7 @@ let pts_to_view
 : Tot vprop
 = VUnit (pts_to_view' r vw)
 
-let pts_to_view_intro_lemma
-  (#a: Type u#0) (#b: Type u#b) (#p: pcm b)
-  (r: ref a p)
-  (x: Ghost.erased b)
-  (#c: Type0)
-  (#can_view_unit: bool)
-  (vw: sel_view p c can_view_unit)
-  (y: Ghost.erased c) // necessary because to_view may erase information from x
-  (m: M.mem)
-: Lemma
-  (requires (M.interp (hp_of (pts_to r x)) m) /\ vw.to_carrier y == Ghost.reveal x)
-  (ensures (
-    M.interp (pts_to_view_sl r vw) m /\
-    pts_to_view_sel r vw m == Ghost.reveal y
-  )) 
-=
-  M.intro_h_exists y (pts_to_view_explicit r vw) m;
-  pts_to_view_explicit_witinv r vw
-
-let pts_to_view_intro
+val pts_to_view_intro
   (#invs: _)
   (#a: Type u#0) (#b: Type u#b) (#p: pcm b)
   (r: ref a p)
@@ -330,50 +251,8 @@ let pts_to_view_intro
     (fun _ _ h' ->
       h' (pts_to_view r vw) == Ghost.reveal y
     )
-= A.change_slprop_2
-    (pts_to r x)
-    (pts_to_view r vw)
-    y
-    (fun m ->
-      pts_to_view_intro_lemma r x vw y m
-    )
 
-let pts_to_view_elim_lemma
-  (#a: Type u#0) (#b: Type u#b) (#p: pcm b)
-  (r: ref a p)
-  (#c: Type0)
-  (#can_view_unit: bool)
-  (vw: sel_view p c can_view_unit)
-  (m: M.mem)
-: Lemma
-  (requires (M.interp (pts_to_view_sl r vw) m))
-  (ensures (
-    M.interp (hp_of (pts_to r (vw.to_carrier (pts_to_view_sel r vw m)))) m
-  ))
-=
-  M.elim_h_exists (pts_to_view_explicit r vw) m;
-  pts_to_view_explicit_witinv r vw
-
-/// Introducing a dependent star for [v] and [q]
-let intro_vdep2 (#opened:_)
-  (v: vprop)
-  (q: vprop)
-  (p: (t_of v -> Tot vprop))
-  (x: t_of v)
-: A.SteelGhost unit opened
-    (v `star` q)
-    (fun _ -> vdep v p)
-    (requires (fun h -> h v == x /\ q == p x))
-    (ensures (fun h _ h' ->
-      let x2 = h' (vdep v p) in
-      q == p (h v) /\
-      dfst x2 == (h v) /\
-      dsnd x2 == (h q)
-    ))
-=
-  A.intro_vdep v q p
-
-let pts_to_view_elim
+val pts_to_view_elim
   (#invs: _)
   (#a: Type u#0) (#b: Type u#b) (#p: pcm b)
   (r: ref a p)
@@ -389,40 +268,8 @@ let pts_to_view_elim
       vw.to_view_prop res /\
       True //~ (Ghost.reveal res == one p)
     )
-=
-  let g : Ghost.erased c = A.gget (pts_to_view r vw) in
-  let res : Ghost.erased b = Ghost.hide (vw.to_carrier g) in
-  // vw.to_carrier_not_one g;
-  A.intro_pure (vw.to_carrier (Ghost.reveal g) == Ghost.reveal res);
-  let f (x: t_of (pts_to_view r vw)) : Tot vprop = pure (vw.to_carrier x == Ghost.reveal res) in
-  intro_vdep2
-    (pts_to_view r vw)
-    (pure (vw.to_carrier (Ghost.reveal g) == Ghost.reveal res))
-    f
-    (Ghost.reveal g);
-  A.rewrite_slprop
-    (vdep (pts_to_view r vw) f)
-    (pts_to r res)
-    (fun m ->
-      interp_vdep_hp (pts_to_view r vw) f m;
-      M.interp_star (hp_of (pts_to_view r vw)) (hp_of (f (sel_of (pts_to_view r vw) m))) m;
-      M.pure_interp (vw.to_carrier (sel_of (pts_to_view r vw) m) == Ghost.reveal res) m;
-      pts_to_view_elim_lemma r vw m
-    );
-  res
 
-let compatible_elim'
-  (#a: Type u#a)
-  (pcm: pcm0 a)
-  (x y: a)
-  (sq: squash (compatible pcm x y))
-: GTot (frame: a {
-    composable pcm x frame /\
-    op pcm frame x == y
-  })
-= compatible_elim pcm x y
-
-let ref_read_sel
+val ref_read_sel
   (#a: Type u#0) (#b: Type u#b) (#p: pcm b)
   (r: ref a p)
   (#c: Type0)
@@ -436,14 +283,5 @@ let ref_read_sel
     res == h (pts_to_view r vw) /\
     res == h' (pts_to_view r vw)
   ))
-=
-  let _v = pts_to_view_elim r vw in
-  let v = ref_read r in
-  let sq : squash (compatible p _v v) = () in
-  let frame = Ghost.hide (compatible_elim' p _v v sq) in
-  vw.to_view_frame (vw.to_view _v) frame ;
-  let res = vw.to_view v in
-  pts_to_view_intro r _v vw res;
-  A.return res
 
 (* write cannot be defined generically because of p_refine *)
